SizeLemmas.v
@@ -6,66 +6,66 @@ Require Import Omega.
 
 (* measure for ensuring termination of reducible_values *)
 (* see file ReducibilityMeasure for the full measure *)
-Fixpoint size T: nat :=
+Fixpoint typeNodes T: nat :=
   match T with
   | T_unit => 0
   | T_bool => 0
   | T_nat => 0
-  | T_refine A p => 1 + size A
-  | T_type_refine A B => 1 + size A + size B
-  | T_arrow A B => 1 + size A + size B
-  | T_prod A B => 1 + size A + size B
-  | T_sum A B => 1 + size A + size B
-  | T_let t B => 1 + size B
+  | T_refine A p => 1 + typeNodes A
+  | T_type_refine A B => 1 + typeNodes A + typeNodes B
+  | T_arrow A B => 1 + typeNodes A + typeNodes B
+  | T_prod A B => 1 + typeNodes A + typeNodes B
+  | T_sum A B => 1 + typeNodes A + typeNodes B
+  | T_let t B => 1 + typeNodes B
   | T_singleton t => 0
-  | T_intersection A B => 1 + size A + size B
-  | T_union A B => 1 + size A + size B
+  | T_intersection A B => 1 + typeNodes A + typeNodes B
+  | T_union A B => 1 + typeNodes A + typeNodes B
   | T_top => 0
   | T_bot => 0
   | T_equal _ _ => 0
-  | T_forall A B => 1 + size A + size B
-  | T_exists A B => 1 + size A + size B
-  | T_abs T => 1 + size T
-  | T_rec _ T0 Ts => 1 + size T0 + size Ts
+  | T_forall A B => 1 + typeNodes A + typeNodes B
+  | T_exists A B => 1 + typeNodes A + typeNodes B
+  | T_abs T => 1 + typeNodes T
+  | T_rec _ T0 Ts => 1 + typeNodes T0 + typeNodes Ts
 
   | _ => 0
   end.
 
-Lemma size_term_form:
-  forall t, is_erased_term t -> size t = 0.
+Lemma typeNodes_term_form:
+  forall t, is_erased_term t -> typeNodes t = 0.
 Proof.
   destruct t; steps.
 Qed.
 
-Lemma size_opening:
-  forall T k rep, is_erased_term rep -> size (open k T rep) = size T.
+Lemma typeNodes_opening:
+  forall T k rep, is_erased_term rep -> typeNodes (open k T rep) = typeNodes T.
 Proof.
-  induction T; repeat step || rewrite_any || apply size_term_form;
+  induction T; repeat step || rewrite_any || apply typeNodes_term_form;
     try omega.
 Qed.
 
-Hint Rewrite size_opening: bsize.
+Hint Rewrite typeNodes_opening: bsize.
 
-Lemma size_opening_var:
-  forall T k X, size (open k T (fvar X type_var)) = size T.
+Lemma typeNodes_opening_var:
+  forall T k X, typeNodes (open k T (fvar X type_var)) = typeNodes T.
 Proof.
   induction T; steps.
 Qed.
 
-Hint Rewrite size_opening_var: bsize.
+Hint Rewrite typeNodes_opening_var: bsize.
 
-Lemma size_topening_var:
-  forall T k X, size (topen k T (fvar X type_var)) = size T.
+Lemma typeNodes_topening_var:
+  forall T k X, typeNodes (topen k T (fvar X type_var)) = typeNodes T.
 Proof.
   induction T; steps.
 Qed.
 
-Hint Rewrite size_topening_var: bsize.
+Hint Rewrite typeNodes_topening_var: bsize.
 
-Lemma size_swap:
-  forall t i j, size (swap_type_holes t i j) = size t.
+Lemma typeNodes_swap:
+  forall t i j, typeNodes (swap_type_holes t i j) = typeNodes t.
 Proof.
   induction t; steps.
 Qed.
 
-Hint Rewrite size_swap: bsize.
+Hint Rewrite typeNodes_swap: bsize.
