TypeOperations.v
@@ -1,74 +1,74 @@
 Require Import SystemFR.Trees.
 
-Inductive T_ite (b: tree): tree -> tree -> tree -> Prop :=
+Inductive T_ite_push (b: tree): tree -> tree -> tree -> Prop :=
 | IteUnit:
-    T_ite b T_unit T_unit T_unit
+    T_ite_push b T_unit T_unit T_unit
 | IteBool:
-    T_ite b T_bool T_bool T_bool
+    T_ite_push b T_bool T_bool T_bool
 | IteNat:
-    T_ite b T_nat T_nat T_nat
+    T_ite_push b T_nat T_nat T_nat
 | IteRefine:
     forall t1 t2 T1 T2 T,
-      T_ite b T1 T2 T ->
-      T_ite b (T_refine T1 t1) (T_refine T2 t2) (T_refine T (ite b t1 t2))
+      T_ite_push b T1 T2 T ->
+      T_ite_push b (T_refine T1 t1) (T_refine T2 t2) (T_refine T (ite b t1 t2))
 | IteProd:
     forall A1 A2 A B1 B2 B,
-      T_ite b A1 A2 A ->
-      T_ite b B1 B2 B ->
-      T_ite b (T_prod A1 B1) (T_prod A2 B2) (T_prod A B)
+      T_ite_push b A1 A2 A ->
+      T_ite_push b B1 B2 B ->
+      T_ite_push b (T_prod A1 B1) (T_prod A2 B2) (T_prod A B)
 | IteArrow:
     forall A1 A2 A B1 B2 B,
-      T_ite b A1 A2 A ->
-      T_ite b B1 B2 B ->
-      T_ite b (T_arrow A1 B1) (T_arrow A2 B2) (T_arrow A B)
+      T_ite_push b A1 A2 A ->
+      T_ite_push b B1 B2 B ->
+      T_ite_push b (T_arrow A1 B1) (T_arrow A2 B2) (T_arrow A B)
 | IteSum:
     forall A1 A2 A B1 B2 B,
-      T_ite b A1 A2 A ->
-      T_ite b B1 B2 B ->
-      T_ite b (T_sum A1 B1) (T_sum A2 B2) (T_sum A B)
+      T_ite_push b A1 A2 A ->
+      T_ite_push b B1 B2 B ->
+      T_ite_push b (T_sum A1 B1) (T_sum A2 B2) (T_sum A B)
 | IteTLet:
     forall B1 B2 B t1 t2,
-      T_ite b B1 B2 B ->
-      T_ite b (T_let t1 B1) (T_let t2 B2) (T_let (ite b t1 t2) B)
+      T_ite_push b B1 B2 B ->
+      T_ite_push b (T_let t1 B1) (T_let t2 B2) (T_let (ite b t1 t2) B)
 | IteSingleton:
     forall t t',
-      T_ite b (T_singleton t) (T_singleton t') (T_singleton (ite b t t'))
+      T_ite_push b (T_singleton t) (T_singleton t') (T_singleton (ite b t t'))
 | IteIntersection:
     forall A1 A2 A B1 B2 B,
-      T_ite b A1 A2 A ->
-      T_ite b B1 B2 B ->
-      T_ite b (T_intersection A1 B1) (T_intersection A2 B2) (T_intersection A B)
+      T_ite_push b A1 A2 A ->
+      T_ite_push b B1 B2 B ->
+      T_ite_push b (T_intersection A1 B1) (T_intersection A2 B2) (T_intersection A B)
 | IteUnion:
     forall A1 A2 A B1 B2 B,
-      T_ite b A1 A2 A ->
-      T_ite b B1 B2 B ->
-      T_ite b (T_union A1 B1) (T_union A2 B2) (T_union A B)
+      T_ite_push b A1 A2 A ->
+      T_ite_push b B1 B2 B ->
+      T_ite_push b (T_union A1 B1) (T_union A2 B2) (T_union A B)
 
 | IteTop:
-    T_ite b T_top T_top T_top
+    T_ite_push b T_top T_top T_top
 | IteBot:
-    T_ite b T_bot T_bot T_bot
+    T_ite_push b T_bot T_bot T_bot
 
 | IteEqual:
     forall u1 v1 u2 v2,
-      T_ite b (T_equal u1 v1) (T_equal u2 v2) (T_equal (ite b u1 u2) (ite b v1 v2))
+      T_ite_push b (T_equal u1 v1) (T_equal u2 v2) (T_equal (ite b u1 u2) (ite b v1 v2))
 
 | IteForall:
     forall A1 A2 A B1 B2 B,
-      T_ite b A1 A2 A ->
-      T_ite b B1 B2 B ->
-      T_ite b (T_forall A1 B1) (T_forall A2 B2) (T_forall A B)
+      T_ite_push b A1 A2 A ->
+      T_ite_push b B1 B2 B ->
+      T_ite_push b (T_forall A1 B1) (T_forall A2 B2) (T_forall A B)
 | IteExists:
     forall A1 A2 A B1 B2 B,
-      T_ite b A1 A2 A ->
-      T_ite b B1 B2 B ->
-      T_ite b (T_exists A1 B1) (T_exists A2 B2) (T_exists A B)
+      T_ite_push b A1 A2 A ->
+      T_ite_push b B1 B2 B ->
+      T_ite_push b (T_exists A1 B1) (T_exists A2 B2) (T_exists A B)
 | IteAbs:
     forall T1 T2 T,
-      T_ite b T1 T2 T ->
-      T_ite b (T_abs T1) (T_abs T2) (T_abs T)
+      T_ite_push b T1 T2 T ->
+      T_ite_push b (T_abs T1) (T_abs T2) (T_abs T)
 | IteTRec:
     forall n1 T01 Ts1 n2 T02 Ts2 T0 Ts,
-      T_ite b T01 T02 T0 ->
-      T_ite b Ts1 Ts2 Ts ->
-      T_ite b (T_rec n1 T01 Ts1) (T_rec n2 T02 Ts2) (T_rec (ite b n1 n2) T0 Ts).
+      T_ite_push b T01 T02 T0 ->
+      T_ite_push b Ts1 Ts2 Ts ->
+      T_ite_push b (T_rec n1 T01 Ts1) (T_rec n2 T02 Ts2) (T_rec (ite b n1 n2) T0 Ts).
