ReducibilitySugar.v
@@ -1,0 +1,91 @@
+Require Import SystemFR.ReducibilityDefinition.
+Require Import SystemFR.ReducibilityLemmas.
+Require Import SystemFR.ReducibilityRefineRules.
+Require Import SystemFR.ReducibilityTypeRefineRules.
+Require Import SystemFR.ReducibilityLetRules.
+Require Import SystemFR.ReducibilitySetOpsRules.
+Require Import SystemFR.ReducibilityCandidate.
+
+Require Import SystemFR.RedTactics.
+Require Import SystemFR.RedTactics2.
+
+Require Import SystemFR.Trees.
+Require Import SystemFR.TypeSugar.
+Require Import SystemFR.Sets.
+Require Import SystemFR.Syntax.
+Require Import SystemFR.AssocList.
+Require Import SystemFR.Tactics.
+Require Import SystemFR.TermList.
+Require Import SystemFR.SmallStep.
+Require Import SystemFR.StarRelation.
+Require Import SystemFR.Equivalence.
+Require Import SystemFR.ListUtils.
+
+Require Import SystemFR.WFLemmas.
+
+Require Import Coq.Lists.List.
+
+Lemma open_reducible_T_ite:
+  forall tvars gamma T1 T2 b t1 t2 x,
+    wf t1 0 ->
+    wf t2 0 ->
+    wf T1 0 ->
+    wf T2 0 ->
+    is_erased_term t1 ->
+    is_erased_term t2 ->
+    is_erased_type T1 ->
+    is_erased_type T2 ->
+    subset (fv t1) (support gamma) ->
+    subset (fv t2) (support gamma) ->
+    subset (fv T1) (support gamma) ->
+    subset (fv T2) (support gamma) ->
+    ~(x ∈ fv b) ->
+    ~(x ∈ fv t1) ->
+    ~(x ∈ fv t2) ->
+    ~(x ∈ fv T1) ->
+    ~(x ∈ fv T2) ->
+    ~(x ∈ fv_context gamma) ->
+    ~(x ∈ tvars) ->
+    is_erased_term b ->
+    is_erased_term t1 ->
+    is_erased_term t2 ->
+    open_reducible tvars gamma b T_bool ->
+    open_reducible tvars ((x, T_equal b ttrue) :: gamma) t1 T1 ->
+    open_reducible tvars ((x, T_equal b tfalse) :: gamma) t2 T2 ->
+    open_reducible tvars gamma (ite b t1 t2) (T_ite b T1 T2).
+Proof.
+  unfold open_reducible; repeat step || t_instantiate_sat3.
+  repeat apply reducible_union || step || top_level_unfold || simp_red.
+
+  - left.
+    apply reducible_refine; repeat step || (rewrite open_none by eauto with bwf);
+      eauto with bwf;
+      eauto with berased;
+      eauto with b_equiv.
+
+    eapply star_backstep_reducible; repeat step || t_listutils; eauto with bsteplemmas;
+      eauto with bfv;
+      eauto with bwf;
+      eauto with berased.
+
+    eapply backstep_reducible; eauto with smallstep; repeat step || t_listutils;
+      eauto with bfv bwf berased.
+
+    unshelve epose proof (H22 theta ((x, uu) :: lterms) _ _); tac1.
+
+  - right.
+    apply reducible_refine; repeat step || (rewrite open_none by eauto with bwf);
+      eauto with bwf;
+      eauto with berased;
+      eauto with b_equiv.
+
+    eapply star_backstep_reducible; repeat step || t_listutils; eauto with bsteplemmas;
+      eauto with bfv;
+      eauto with bwf;
+      eauto with berased.
+
+    eapply backstep_reducible; eauto with smallstep; repeat step || t_listutils;
+      eauto with bfv bwf berased.
+
+    unshelve epose proof (H23 theta ((x, uu) :: lterms) _ _); tac1.
+Qed.
