SomeTerms.v
@@ -9,3 +9,7 @@ Definition tpred (a: tree): tree :=
 
 Definition notype_tpred (a: tree): tree :=
   tmatch a notype_err (lvar 0 term_var).
+
+Definition negate (t: tree): tree := ite t tfalse ttrue.
+Definition unfold_left (t: tree): tree := sum_match t (lvar 0 term_var) notype_err.
+Definition unfold_right (t: tree): tree := sum_match t notype_err (lvar 0 term_var).
