TypeOperationsLemmas.v
@@ -15,10 +15,10 @@ Require Import SystemFR.TypeOperations.
 Require Import SystemFR.ListUtils.
 
 Lemma ite_type_open:
-  forall b T1 T2 T, T_ite b T1 T2 T -> forall k a,
+  forall b T1 T2 T, T_ite_push b T1 T2 T -> forall k a,
     is_erased_term a ->
     wf b 0 ->
-    T_ite b (open k T1 a) (open k T2 a) (open k T a).
+    T_ite_push b (open k T1 a) (open k T2 a) (open k T a).
 Proof.
   induction 1; repeat step || constructor || t_fv_open || t_listutils ||
                       rewrite (open_none b) in * by (eauto with bwf omega) ||
@@ -27,9 +27,9 @@ Proof.
 Qed.
 
 Lemma ite_type_topen:
-  forall b T1 T2 T, T_ite b T1 T2 T -> forall k X,
+  forall b T1 T2 T, T_ite_push b T1 T2 T -> forall k X,
     twf b 0 ->
-    T_ite b (topen k T1 (fvar X type_var)) (topen k T2 (fvar X type_var)) (topen k T (fvar X type_var)).
+    T_ite_push b (topen k T1 (fvar X type_var)) (topen k T2 (fvar X type_var)) (topen k T (fvar X type_var)).
 Proof.
   induction 1; repeat step || constructor || t_fv_open || t_listutils ||
                       rewrite (topen_none b) in * by (eauto with btwf omega) ||
@@ -38,8 +38,8 @@ Proof.
 Qed.
 
 Lemma ite_type_subst:
-  forall b T1 T2 T, T_ite b T1 T2 T -> forall l,
-    T_ite (psubstitute b l term_var) (psubstitute T1 l term_var) (psubstitute T2 l term_var) (psubstitute T l term_var).
+  forall b T1 T2 T, T_ite_push b T1 T2 T -> forall l,
+    T_ite_push (psubstitute b l term_var) (psubstitute T1 l term_var) (psubstitute T2 l term_var) (psubstitute T l term_var).
 Proof.
   induction 1; repeat step || constructor.
 Qed.
